### Breakdown of the Solution:

1. **Base Cases**: If `n` is 1 or 2, the function returns `1`.

2. **Recursive Case**: For all other `n`, the function returns the sum of `fibonacci(n-1)` and `fibonacci(n-2)`.

### The Call Stack:

To understand the call stack better, let's visualize it with a smaller input, say, `fibonacci(4)`:

1. The initial call is `fibonacci(4)`.

2. This expands to:
   - `fibonacci(2)` + `fibonacci(3)`
     - `fibonacci(2)` directly returns `1` due to the base case.
     - `fibonacci(3)` expands further to:
       - `fibonacci(1)` + `fibonacci(2)`
         - Both `fibonacci(1)` and `fibonacci(2)` directly return `1` due to the base case.

### Call Stack Visualization:

```
fibonacci(4)
    |
    |--> fibonacci(2) // Returns 1
    |
    |--> fibonacci(3)
    |       |
    |       |--> fibonacci(1) // Returns 1
    |       |
    |       |--> fibonacci(2) // Returns 1
    |
    |-----> Result: 1 + (1 + 1) = 3
```

